theories/goedel/PRrepresentable.v
@@ -176,7 +176,7 @@ Proof.
                         rewrite subTermNil.
                         **** (* fold (var 4) in |- *. *)
                              replace 
-                               (apply LNN Languages.Succ 
+                               (apply LNN Languages.Succ_ 
                                   (Tcons (natToTerm a)
                                      (Tnil)))
                                with (natToTerm (S a)); 
@@ -248,10 +248,10 @@ Proof.
                                  * apply Axm; right; constructor.
                                  * apply sysWeaken.
                                    replace
-                                     (apply LNN Languages.Succ
-                                        (Tcons (apply LNN Languages.Succ
+                                     (apply LNN Languages.Succ_
+                                        (Tcons (apply LNN Languages.Succ_
                                               (Tcons 
-                                                 (apply LNN Languages.Zero
+                                                 (apply LNN Languages.Zero_
                                                     (Tnil))
                                                  (Tnil)))
                                            (Tnil)))
@@ -409,12 +409,12 @@ Proof.
                                                              (Tcons                                                                 (apply LNN Languages.Times_
                                                                    (Tcons (var  5)
                                                                       (Tcons 
-                                                                         (apply LNN Languages.Succ
+                                                                         (apply LNN Languages.Succ_
                                                                             (Tcons 
                                                                                (apply LNN Languages.Times_
                                                                                   (Tcons  (natToTerm (cPairPi1 a))
                                                                                      (Tcons 
-                                                                                        (apply LNN Languages.Succ
+                                                                                        (apply LNN Languages.Succ_
                                                                                            (Tcons  
                                                                                               (natToTerm a0) 
                                                                                               (Tnil))) 
@@ -449,12 +449,12 @@ Proof.
                                                                        (apply LNN Languages.Times_
                                                                           (Tcons  (natToTerm n0)
                                                                              (Tcons 
-                                                                                (apply LNN Languages.Succ
+                                                                                (apply LNN Languages.Succ_
                                                                                    (Tcons 
                                                                                       (apply LNN Languages.Times_
                                                                                          (Tcons  (natToTerm (cPairPi1 a))
                                                                                             (Tcons 
-                                                                                               (apply LNN Languages.Succ
+                                                                                               (apply LNN Languages.Succ_
                                                                                                   (Tcons (natToTerm a0) (Tnil)))
                                                                                                (Tnil )))) (Tnil ))) 
                                                                                 (Tnil )))) (Tnil )))) with
@@ -494,7 +494,7 @@ Proof.
         induction x as (a1, b). simpl in |- *. simpl in H1. destruct H1 as (H1, H2).
         apply existI with (natToTerm (cPairPi1 a)). rewrite (subFormulaAnd LNN). apply andI.
         -- apply sysWeaken. rewrite H0. simpl in |- *. rewrite subTermNil.
-           ++ replace (apply LNN Languages.Succ (Tcons (natToTerm a) (Tnil ))) with (natToTerm (S a)) by reflexivity.
+           ++ replace (apply LNN Languages.Succ_ (Tcons (natToTerm a) (Tnil ))) with (natToTerm (S a)) by reflexivity.
               apply natLT. apply Nat.lt_succ_r. apply Nat.le_trans with (cPair (cPairPi1 a) (cPairPi2 a)).
               apply cPairLe1. rewrite cPairProjections. apply le_n.
            ++ apply closedNatToTerm.
@@ -502,7 +502,7 @@ Proof.
            ++ apply existI with (natToTerm (cPairPi2 a)). repeat rewrite (subFormulaAnd LNN). apply andI.
               ** apply sysWeaken. repeat rewrite H0. simpl in |- *.
                  repeat rewrite (subTermNil LNN (natToTerm a)).
-                 --- replace (apply LNN Languages.Succ (Tcons (natToTerm a) (Tnil ))) with (natToTerm (S a))
+                 --- replace (apply LNN Languages.Succ_ (Tcons (natToTerm a) (Tnil ))) with (natToTerm (S a))
                        by reflexivity.
                      apply natLT. apply Nat.lt_succ_r. apply Nat.le_trans with (cPair (cPairPi1 a) (cPairPi2 a)).
                      +++ apply cPairLe2.
@@ -526,7 +526,7 @@ Proof.
                                         (Tcons (natToTerm (cPairPi1 a))
                                            (Tcons (natToTerm (cPairPi2 a)) (Tnil ))))
                                      (Tcons
-                                        (apply LNN Languages.Succ
+                                        (apply LNN Languages.Succ_
                                            (Tcons
                                               (apply LNN Languages.Plus_
                                                  (Tcons (natToTerm (cPairPi1 a))
@@ -536,20 +536,21 @@ Proof.
                                (Tcons
                                   (apply LNN Languages.Times_
                                      (Tcons
-                                        (apply LNN Languages.Succ
+                                        (apply LNN Languages.Succ_
                                            (Tcons
-                                              (apply LNN Languages.Succ
+                                              (apply LNN Languages.Succ_
                                                  (Tcons
-                                                    (apply LNN Languages.Zero (Tnil ))
+                                                    (apply LNN 
+                                                       Languages.Zero_ (Tnil ))
                                                     (Tnil ))) (Tnil )))
                                         (Tcons (natToTerm (cPairPi1 a)) (Tnil ))))
                                   (Tnil ))))
                          (apply LNN Languages.Times_
                             (Tcons
-                               (apply LNN Languages.Succ
+                               (apply LNN Languages.Succ_
                                   (Tcons
-                                     (apply LNN Languages.Succ
-                                        (Tcons (apply LNN Languages.Zero (Tnil ))
+                                     (apply LNN Languages.Succ_
+                                        (Tcons (apply LNN Languages.Zero_ (Tnil ))
                                            (Tnil ))) (Tnil )))
                                (Tcons (natToTerm a) (Tnil ))))) with
                       (equal
@@ -667,7 +668,7 @@ Proof.
                              repeat
                               (rewrite (subTermNil LNN (natToTerm a1)); [| apply closedNatToTerm ]).
                              apply andI.
-                             ---- replace (apply LNN Languages.Succ (Tcons (natToTerm (cPairPi2 a)) (Tnil ))) 
+                             ---- replace (apply LNN Languages.Succ_ (Tcons (natToTerm (cPairPi2 a)) (Tnil ))) 
                                     with (natToTerm (S (cPairPi2 a))) by reflexivity.
                                   apply natLT. unfold coPrimeBeta in *. lia.
                              ---- replace
@@ -677,12 +678,12 @@ Proof.
                                             (apply LNN Languages.Times_
                                                (Tcons (natToTerm a1)
                                                   (Tcons
-                                                     (apply LNN Languages.Succ
+                                                     (apply LNN Languages.Succ_
                                                         (Tcons
                                                            (apply LNN Languages.Times_
                                                               (Tcons (natToTerm (cPairPi1 a))
                                                                  (Tcons
-                                                                    (apply LNN Languages.Succ
+                                                                    (apply LNN Languages.Succ_
                                                                        (Tcons (natToTerm a0) (Tnil )))
                                                                     (Tnil )))) (Tnil ))) 
                                                      (Tnil )))) (Tnil )))) with
